src/3d/ParserDriver.fsti
@@ -1,5 +1,5 @@
 module ParserDriver
 open FStar.All
 open Ast
-val parse (filename:string) : ML (list decl)
+val parse (filename:string) : ML prog
 val int_of_string (x:string) : ML int
